replace lift_' lift_3 ... with syntax lambda_T ...

DP_Lifting.thy
@@ -35,15 +35,12 @@ abbreviation checkmem_eq :: "('param \<Rightarrow>\<^sub>T 'result) \<Rightarrow
 term 0 (**)
   
   (* Auxiliary *)
-definition lift_' :: "'a \<Rightarrow> 'a" where
-  "lift_' x \<equiv> x"
-definition lift_3 :: "('a \<Rightarrow> 'b) \<Rightarrow> ('a =='M\<Longrightarrow> 'b)" where
-  "lift_3 f \<equiv> \<lambda>v. \<langle>lift_' (f v)\<rangle>"
-definition lift_33 :: "('a \<Rightarrow> 'b \<Rightarrow> 'c) \<Rightarrow> ('a =='M\<Longrightarrow> 'b =='M\<Longrightarrow> 'c)" where
-  "lift_33 f \<equiv> \<lambda>v. \<langle>lift_3 (f v)\<rangle>"
-definition lift_333 :: "('a \<Rightarrow> 'b \<Rightarrow> 'c \<Rightarrow> 'd) \<Rightarrow> ('a =='M\<Longrightarrow> 'b =='M\<Longrightarrow> 'c =='M\<Longrightarrow> 'd)" where
-  "lift_333 f \<equiv> \<lambda>v. \<langle>lift_33 (f v)\<rangle>"
-  
+syntax
+  "_lambda\<^sub>T" :: "[pttrns, 'a] \<Rightarrow> logic" ("(3\<lambda>\<^sub>T_./ _)" [0, 3] 3)
+translations
+  "\<lambda>\<^sub>T v vs. e" \<rightharpoonup> "\<lambda> v. \<langle>\<lambda>\<^sub>T vs. e\<rangle>"
+  "\<lambda>\<^sub>T v. e" \<rightharpoonup> "\<lambda> v. \<langle>e\<rangle>"
+
 definition unlift_' :: "'a \<Rightarrow> ('M, 'a) state" where
   "unlift_' x \<equiv> \<langle>x\<rangle>"
 definition unlift_3 :: "('a =='M\<Longrightarrow> 'b) \<Rightarrow> ('a \<Rightarrow> ('M, 'b) state)" where
@@ -55,23 +52,23 @@ term 0 (**)
   
   (* HOL *)
 definition If\<^sub>T :: "bool =='M\<Longrightarrow> 'a =='M\<Longrightarrow> 'a =='M\<Longrightarrow> 'a" where
-  "If\<^sub>T \<equiv> lift_333 If"
-  
+  "If\<^sub>T \<equiv> \<lambda>\<^sub>T P x y. If P x y"
+
 thm comp_def
 definition comp\<^sub>T :: "('b =='M\<Longrightarrow> 'c) =='M\<Longrightarrow> ('a =='M\<Longrightarrow> 'b) =='M\<Longrightarrow> ('a =='M\<Longrightarrow> 'c)" where
-  "comp\<^sub>T \<equiv> \<lambda>f. \<langle>\<lambda>g. \<langle>\<lambda>x. \<langle>f\<rangle> . (\<langle>g\<rangle> . \<langle>x\<rangle>)\<rangle>\<rangle>"
+  "comp\<^sub>T \<equiv> \<lambda>\<^sub>T f g. (\<lambda>x. \<langle>f\<rangle> . (\<langle>g\<rangle> . \<langle>x\<rangle>))"
   
 thm id_def
 definition id\<^sub>T :: "'a =='M\<Longrightarrow> 'a" where
-  "id\<^sub>T \<equiv> \<lambda>x. \<langle>x\<rangle>"
+  "id\<^sub>T \<equiv> \<lambda>\<^sub>T x. x"
 term 0 (**)
   
   (* List *)
 definition Cons\<^sub>T :: "'a =='M\<Longrightarrow> 'a list =='M\<Longrightarrow> 'a list" where
-  "Cons\<^sub>T \<equiv> lift_33 Cons"
+  "Cons\<^sub>T \<equiv> \<lambda>\<^sub>T x xs. Cons x xs"
   
 definition case_list\<^sub>T :: "'b =='M\<Longrightarrow> ('a =='M\<Longrightarrow> 'a list =='M\<Longrightarrow> 'b) =='M\<Longrightarrow> 'a list =='M\<Longrightarrow> 'b" where
-  "case_list\<^sub>T \<equiv> \<lambda>ifNil. \<langle>\<lambda>ifCons. \<langle>\<lambda>val. case_list (unlift_' ifNil) (unlift_33 ifCons) val\<rangle>\<rangle>"
+  "case_list\<^sub>T \<equiv> \<lambda>\<^sub>T ifNil ifCons. (\<lambda>val. case_list (unlift_' ifNil) (unlift_33 ifCons) val)"
   
 primrec map\<^sub>T' :: "('a =='M\<Longrightarrow>'b) \<Rightarrow> 'a list =='M\<Longrightarrow> 'b list" where
   "(map\<^sub>T' f) [] = \<langle>[]\<rangle>"
@@ -80,7 +77,7 @@ lemma
   "(map\<^sub>T' f) (x#xs) = \<langle>Cons\<^sub>T\<rangle> . (\<langle>f\<rangle> . \<langle>x\<rangle>) . (\<langle>map\<^sub>T' f\<rangle> . \<langle>xs\<rangle>)" unfolding map\<^sub>T'.simps(2) fun_app_lifted_def left_identity ..
     
 definition map\<^sub>T :: "('a =='M\<Longrightarrow> 'b) =='M\<Longrightarrow> 'a list =='M\<Longrightarrow> 'b list" where
-  "map\<^sub>T \<equiv> lift_3 map\<^sub>T'"
+  "map\<^sub>T \<equiv> \<lambda>\<^sub>T f\<^sub>T. map\<^sub>T' f\<^sub>T"
   
 primrec fold\<^sub>T' :: "('a =='M\<Longrightarrow> 'b =='M\<Longrightarrow> 'b) \<Rightarrow> 'a list =='M\<Longrightarrow> 'b =='M\<Longrightarrow> 'b" where
   "(fold\<^sub>T' f) [] = \<langle>id\<^sub>T\<rangle>"
@@ -89,38 +86,38 @@ lemma
   "(fold\<^sub>T' f) (x#xs) = \<langle>comp\<^sub>T\<rangle> . (\<langle>fold\<^sub>T' f\<rangle> . \<langle>xs\<rangle>) . (\<langle>f\<rangle> . \<langle>x\<rangle>)" unfolding fold\<^sub>T'.simps(2) fun_app_lifted_def left_identity ..
     
 definition fold\<^sub>T :: "('a =='M\<Longrightarrow> 'b =='M\<Longrightarrow> 'b) =='M\<Longrightarrow> 'a list =='M\<Longrightarrow> 'b =='M\<Longrightarrow> 'b" where
-  "fold\<^sub>T \<equiv> lift_3 fold\<^sub>T'"
+  "fold\<^sub>T \<equiv> \<lambda>\<^sub>T f\<^sub>T. fold\<^sub>T' f\<^sub>T"
 
 definition upt\<^sub>T :: "nat =='M\<Longrightarrow> nat =='M\<Longrightarrow> nat list" where
-  "upt\<^sub>T \<equiv> lift_33 upt"
+  "upt\<^sub>T \<equiv> \<lambda>\<^sub>T i j. upt i j"
 term 0 (**)
   
   (* Option *)
 definition Some\<^sub>T :: "'a =='M\<Longrightarrow> 'a option" where
-  "Some\<^sub>T \<equiv> lift_3 Some"
+  "Some\<^sub>T \<equiv> \<lambda>\<^sub>T x. Some x"
   
 definition case_option\<^sub>T :: "'b =='M\<Longrightarrow> ('a =='M\<Longrightarrow> 'b) =='M\<Longrightarrow> 'a option =='M\<Longrightarrow> 'b" where
-  "case_option\<^sub>T \<equiv> \<lambda>ifNone. \<langle>\<lambda>ifSome. \<langle>\<lambda>val. case_option (unlift_' ifNone) (unlift_3 ifSome) val\<rangle>\<rangle>"
+  "case_option\<^sub>T \<equiv> \<lambda>\<^sub>T ifNone ifSome. (\<lambda>val. case_option (unlift_' ifNone) (unlift_3 ifSome) val)"
 term 0 (**)
   
   (* Prod *)
 definition Pair\<^sub>T :: "'a0 =='M\<Longrightarrow> 'a1 =='M\<Longrightarrow> 'a0\<times>'a1" where
-  "Pair\<^sub>T \<equiv> lift_33 Pair"
+  "Pair\<^sub>T \<equiv> \<lambda>\<^sub>T x y. Pair x y"
   
 definition case_prod\<^sub>T :: "('a0 =='M\<Longrightarrow> 'a1 =='M\<Longrightarrow> 'b) =='M\<Longrightarrow> ('a0\<times>'a1) =='M\<Longrightarrow> 'b" where
-  "case_prod\<^sub>T \<equiv> \<lambda>ifProd. \<langle>\<lambda>val. case_prod (unlift_33 ifProd) val\<rangle>"
+  "case_prod\<^sub>T \<equiv> \<lambda>\<^sub>T ifProd. (\<lambda>val. case_prod (unlift_33 ifProd) val)"
   
-term "\<langle>case_prod\<^sub>T\<rangle> . \<langle>\<lambda>v0. \<langle>\<lambda>v1. \<langle>v0+v1\<rangle>\<rangle>\<rangle> . (\<langle>Pair\<^sub>T\<rangle> . \<langle>0\<rangle> . \<langle>0::int\<rangle>)"
+term "\<langle>case_prod\<^sub>T\<rangle> . \<langle>\<lambda>\<^sub>T v0 v1. v0+v1\<rangle> . (\<langle>Pair\<^sub>T\<rangle> . \<langle>0\<rangle> . \<langle>0::int\<rangle>)"
 term 0 (**)
   
   (* Arithmetic *)
 definition min\<^sub>T :: "'a::ord =='M\<Longrightarrow> 'a =='M\<Longrightarrow> 'a" where
-  "min\<^sub>T \<equiv> lift_33 min"
+  "min\<^sub>T \<equiv> \<lambda>\<^sub>T x y. min x y"
   
 definition max\<^sub>T :: "'a::ord =='M\<Longrightarrow> 'a =='M\<Longrightarrow> 'a" where
-  "max\<^sub>T \<equiv> lift_33 max"
+  "max\<^sub>T \<equiv> \<lambda>\<^sub>T x y. max x y"
   
 definition plus\<^sub>T :: "'a::plus =='M\<Longrightarrow> 'a =='M\<Longrightarrow> 'a" where
-  "plus\<^sub>T \<equiv> lift_33 plus"
+  "plus\<^sub>T \<equiv> \<lambda>\<^sub>T x y. plus x y"
 term 0 (**)
 end
